src/Repr/SystemFOp/TypeRel.v
@@ -1,0 +1,260 @@
+Require Import List.
+
+Require Import Repr.Lists.
+
+Require Import Repr.Tactics.All.
+Require Import Repr.Tactics.Rewrite.
+Require Import Repr.Tactics.Burn.
+Require Import Repr.Tactics.Norm.
+Require Import Repr.Tactics.LibTactics.
+
+Require Import Coq.Arith.Peano_dec.
+Require Import Coq.Arith.Compare_dec.
+Require Import Coq.Arith.Lt.
+
+Require Import Repr.SystemFOp.Kind.
+Require Import Repr.SystemFOp.Type.
+Require Import Repr.SystemFOp.Term.
+
+Require Import Repr.Tactics.CpdtTactics.
+
+(* We define the typing relation over kind and type environments. D and G standing
+   for delta and gamma resp. *)
+Reserved Notation "D ',' G '||-' t '\:' T" (at level 40).
+
+Inductive type_rel : kenv -> tenv -> term -> typ -> Prop :=
+  | TR_NConst :
+      forall D G n,
+        D, G ||- (NConst n) \: TNat
+  | TR_Add :
+      forall D G t1 t2,
+        D, G ||- t1 \: TNat ->
+        D, G ||- t2 \: TNat ->
+        D, G ||- (Add t1 t2) \: TNat
+  | TR_Var :
+      forall D G x T,
+        get G x = Some T ->
+        D, G ||- (Var x) \: T 
+  | TR_Abs :
+      forall D G t T1 T2,
+        D, (T1 :: G) ||- t \: T2 ->
+        D, G ||- Abs T1 t \: TArrow T1 T2
+  | TR_App :
+      forall D G t1 t2 T1 T2,
+        D, G ||- t1 \: TArrow T1 T2 ->
+        D, G ||- t2 \: T1 ->
+        D, G ||- App t1 t2 \: T2
+  | TR_TyAbs :
+      forall D G t T,
+        (KStar :: D), (tenv_lift 0 G) ||- t \: T ->
+        D, G ||- (TyAbs t) \: TAll T
+  | TR_TyApp :
+      forall D G t T ty, 
+        D, G ||- t \: TAll T ->
+        D, G ||- (TyApp t ty) \: [0 |=> ty] T
+
+where "D ',' G '||-' t '\:' T" := (type_rel D G t T).
+
+Hint Constructors type_rel.
+
+(********************************************************************)
+(* On to the substitution lemmas. They have more in common with the
+ * typing relation than the proof of soundness, hence, hey remain here. *)
+
+(* Simple tactic that helps burn down the easy cases. *)
+Ltac inverts_type :=
+  repeat
+    (match goal with
+       | [ H: _,_ ||- (NConst _)   \: _ |- _ ] => inverts H
+       | [ H: _,_ ||- (Add _ _)    \: _ |- _ ] => inverts H
+       | [ H: _,_ ||- (Var _)      \: _ |- _ ] => inverts H
+       | [ H: _,_ ||- (Abs _ _)    \: _ |- _ ] => inverts H
+       | [ H: _,_ ||- (App _ _)    \: _ |- _ ] => inverts H
+       | [ H: _,_ ||- (TyAbs _)    \: _ |- _ ] => inverts H
+       | [ H: _,_ ||- (TyApp _ _)  \: _ |- _ ] => inverts H
+     end).
+
+(* This tactic 'usually' gets most of the inductive and easy cases
+ * when we induct over the typing relation. *)
+Tactic Notation "induction_type" ident(t) :=
+  induction t; rip; simpl; inverts_type; tburn.
+
+Lemma get_lift
+  :  forall (G:tenv)(x:var)(T:typ)(X:tvar)
+  ,  get G x = Some T
+  -> get (tenv_lift X G) x = Some (typ_lift X T).
+Proof.
+  induction G; destruct x; rip; 
+  simpl in *; try norm_some; tburn.
+Qed.
+Hint Resolve get_lift.
+
+Lemma rewind_typ_lift
+  :  forall (G:tenv)(T:typ)(X:tvar)
+  ,  typ_lift X T :: tenv_lift X G = tenv_lift X (T :: G).
+Proof. tburn. Qed.
+Hint Rewrite rewind_typ_lift.
+
+(*
+Lemma le_gt_dec_S
+  :  forall n m pf
+  ,  left pf = le_gt_dec n m 
+  -> exists pf', left pf' = le_gt_dec (S n) (S m). 
+Proof. 
+  rip; dep_destruct (le_gt_dec (S n) (S m)); tburn.
+Qed.
+Hint Resolve le_gt_dec_S. *)
+
+Lemma typ_lift_SX
+  :  forall (X Y:tvar)(T:typ)
+  ,  Y <= X
+  -> typ_lift Y (typ_lift X T) = typ_lift (S X) (typ_lift Y T).
+Proof.
+  rip; gen X Y; induction T; tburn.
+
+  rip;
+  rename t into Z;
+  break Z;
+  repeat(
+    simpl;
+    match goal with 
+      | [ |- context[le_gt_dec ?X ?Y] ] =>
+        break (le_gt_dec X Y)
+    end;
+    tburn
+  ).
+Qed.  
+
+Lemma tenv_lift_SX
+  :  forall (G:tenv)(X:tvar)
+  ,  tenv_lift 0 (tenv_lift X G) = tenv_lift (S X) (tenv_lift 0 G).
+Proof.
+  induction G; rip; simpl; tburn.
+  rewrite IHG; rewrite typ_lift_SX; burn.
+Qed.
+
+(* Handy tactic for burning down TVar case analysis which usually boils down
+ * to repeated less than and nat compares *)
+Ltac burn_tvar :=
+  repeat(
+    simpl;
+    break_nat_compare;
+    tburn;
+    match goal with
+      | [ |- context[le_gt_dec ?X ?Y] ] => break (le_gt_dec X Y)
+    end;
+    tburn
+  ).
+
+Lemma tall_injective 
+  :  forall (T1 T2:typ)
+  ,  T1 = T2
+  -> TAll T1 = TAll T2.
+Proof. burn. Qed.
+
+Lemma typ_lift_before_subs
+  :  forall (X Y:tvar)(U T:typ)
+  ,  X <= Y
+  -> typ_lift X ([Y |=> U] T) =  [(S Y) |=> typ_lift X U] typ_lift X T.
+Proof.
+  rip; gen X Y U; induction T; tburn.
+  rip; burn_tvar.
+
+  rip; simpl; eapply tall_injective.
+  rewrite IHT. rewrite <- typ_lift_SX; burn. burn.
+Qed.
+
+Lemma typ_lift_after_subs
+  :  forall (X Y:tvar)(U T:typ)
+  ,  X > Y
+  -> typ_lift X ([Y |=> U] T) =  [Y |=> typ_lift X U] typ_lift X T.
+Proof.
+  rip; gen X Y U; induction T; tburn.
+  rip; burn_tvar.
+  rename t into Z. simpl. break (le_gt_dec X (Z-1)). 
+  
+  
+  
+
+  
+
+  rip; simpl; eapply tall_injective.
+  rewrite IHT. rewrite <- typ_lift_SX; burn. burn.
+Qed.
+
+
+
+Hint Resolve typ_lift_before_subs.
+
+Lemma kenv_weaking
+  :  forall (D:kenv)(G:tenv)(t:term)(T:typ)(X:tvar)
+  ,  delete D X, G ||- t \: T
+  -> D, (tenv_lift X G) ||- (typ_term_lift X t) \: (typ_lift X T).
+Proof.
+  rip; gen D G T X; induction_type t.
+
+  assert (TNat = typ_lift 0 TNat).
+    burn.
+  econstructor; burn.
+
+  simpl.
+  constructor. autorewrite_goal. eapply IHt. assumption.
+
+  simpl.
+  constructor.
+
+  
+  rewrite tenv_lift_SX. eapply IHt. simpl. burn.
+
+  rename t0 into ty.
+
+  
+
+
+
+Qed.  
+
+Lemma tenv_weakening
+  :  forall (D:kenv)(G:tenv)(t:term)(T:typ)(x:var)
+  ,  D, delete G x ||- t \: T
+  -> D, G ||- term_lift x t \: T.
+Proof.
+  rip; gen G T x; induction_type t.
+  match goal with
+    | [ |- context[le_gt_dec ?X ?Y] ] 
+      => break (le_gt_dec X Y); tburn;
+         constructor; rewrite get_delete_above_idx in *; tburn
+  end.
+Qed.
+Hint Resolve env_weakening.
+
+Lemma tm_substition_preserves_typing' 
+  :  forall (G:env)(x:var)(s t:term)(U T:typ)
+  ,  get G x = Some (term,U) 
+  -> delete G x ||- s \: U 
+  -> G ||- t \: T 
+  -> delete G x ||- [x ~> s] t \: T.
+Proof.
+  rip; gen G x s U T; induction_type t;
+  match goal with
+    (* TVar *)
+    | [ |- context [ nat_compare _ _ ] ] 
+      => break_nat_compare; tburn; constructor; tburn
+    (* TAbs *)                                              
+    | [ |- context [ Abs _ ]           ]
+      => econstructor; rewrite delete_rewind; tburn
+  end.
+Qed.
+
+Lemma tm_substition_preserves_typing 
+  :  forall (G:env)(s t:term)(U T:typ)
+  ,  delete ((term,U) :: G) 0 ||- s \: U 
+  -> ((term,U) :: G) ||- t \: T 
+  -> delete ((term,U) :: G) 0 ||- [0 ~> s] t \: T.
+Proof.
+  rip; eapply tm_substition_preserves_typing'; tburn. 
+Qed.
+
+
+
+
